examples/sampler/traffic_manager.v
@@ -1,0 +1,47 @@
+Require Import Poulet4.P4light.Syntax.P4defs.
+Require Import Poulet4.P4light.Semantics.Semantics.
+Require Import ProD3.core.Core.
+Require Import Poulet4.P4light.Architecture.Tofino.
+Require Import Poulet4.P4light.Architecture.TrafficManager.
+Require Import ProD3.core.Tofino.
+Require Import ProD3.core.TofinoPipeline.
+Require Import ProD3.examples.sampler.ModelRepr.
+Require Import ProD3.examples.sampler.common.
+Require Import ProD3.core.ProgNotations.
+Require Import Poulet4.P4light.Syntax.P4Notations.
+Require Import Hammer.Plugin.Hammer.
+Require Export Coq.Program.Program.
+Import ListNotations.
+
+Notation Port := Z (only parsing).
+
+Definition ctrl_node_setting: MulticastLevel1Node Port:=
+  Build_MulticastLevel1Node 123 0 false [129].
+
+Definition excl_table: L2_exclusion_table Port := fun _ => [].
+
+Definition mcast_tbl: multicast_table Port := [(1, [ctrl_node_setting])].
+
+Definition validityP4Bit_to_Z (s: Sval): option Z :=
+  match s with
+  | ValBaseBit l => match lift_option l with
+                   | Some s => match (snd (P4Arith.BitArith.from_lbool s)) with
+                              | 0 => None
+                              | n => Some n
+                              end
+                   | None => None
+                   end
+  | _ => None
+  end.
+
+Definition intr_tm_md_to_input_md (ig_intr_tm_md: Sval): InputMetadata Port :=
+  let ucast_port := get "ucast_egress_port" ig_intr_tm_md in
+  let mcast_grp_a := get "mcast_grp_a" ig_intr_tm_md in
+  let mcast_grp_b := get "mcast_grp_b" ig_intr_tm_md in
+  Build_InputMetadata (validityP4Bit_to_Z ucast_port)
+    (validityP4Bit_to_Z mcast_grp_a)
+    (validityP4Bit_to_Z mcast_grp_b) 0 0 0.
+
+Definition tofino_tm {PT: Type} (ig_intr_tm_md: Sval) (packet: PT) :=
+  traffic_manager mcast_tbl excl_table
+    (intr_tm_md_to_input_md ig_intr_tm_md, packet).
